got obligations finder in place, trying to use it to verify programs are wellformed

theorems/main.v
@@ -1,226 +1,12 @@
-Add LoadPath "/home/blaine/personal/cpdtlib" as Cpdt.
+Add LoadPath "/home/blaine/lab/cpdtlib" as Cpdt.
 Set Implicit Arguments. Set Asymmetric Patterns.
 Require Import List String Cpdt.CpdtTactics Coq.Program.Wf.
 From stdpp Require Import base fin vector options.
 Import ListNotations.
-
-Ltac solve_crush := try solve [crush].
-Ltac solve_assumption := try solve [assumption].
-Ltac subst_injection H := injection H; intros; subst; clear H.
-
-Notation impossible := (False_rect _ _).
-Notation this item := (exist _ item _).
-Notation use item := (proj1_sig item).
-
-Section convert_subset.
-	Variable T: Type.
-	Variable P Q: T -> Prop.
-	Theorem convert_subset: {t | P t} -> (forall t: T, P t -> Q t) -> {t | Q t}.
-	Proof. intros []; eauto. Qed.
-End convert_subset.
-Arguments convert_subset {T} {P} {Q} _ _.
-
-Notation convert item := (convert_subset item _).
-
-Notation Yes := (left _ _).
-Notation No := (right _ _).
-Notation Reduce x := (if x then Yes else No).
-
-
-Inductive partial (P: Prop): Type :=
-	| Done: P -> partial P
-	| Undone: partial P
-.
-Arguments Undone {P}.
-
-Section find_obligations.
-	Context {T: Type}.
-	Variable P: T -> Prop.
-
-	Theorem combine_Done_Undone: forall items done undone,
-		Permutation items (done ++ undone)
-		-> Forall P done -> Forall P undone
-		-> Forall P items.
-	Proof.
-		intros ??? Hpermutation ??; assert (Happ: Forall P (done ++ undone))
-			by solve [apply Forall_app_2; assumption];
-		setoid_rewrite Hpermutation; assumption.
-	Qed.
-
-	Variable compute_partial: forall t: T, partial (P t).
-
-	Definition split_by_maybe: forall items: list T, {
-		pair | Permutation items (pair.1 ++ pair.2) /\ Forall P pair.1
-	}.
-		refine (fix split_by_maybe items :=
-			match items with
-			| [] => this ([], [])
-			| item :: items' =>
-				let (pair, H) := split_by_maybe items' in
-				match (compute_partial item) with
-				| Done _ => this ((item :: pair.1), pair.2)
-				| Undone => this (pair.1, (item :: pair.2))
-				end
-			end
-		);
-		intros; split; simpl in *; try destruct H;
-		try solve [setoid_rewrite H; apply Permutation_middle]; auto.
-	Defined.
-
-	Definition find_obligations_function: forall items, {
-		obligations | Forall P obligations -> Forall P items
-	}.
-		refine (fun items =>
-			let (pair, H) := split_by_maybe items in
-			this pair.2
-		);
-		destruct H; apply (combine_Done_Undone H); assumption.
-	Defined.
-
-	Theorem use_find_obligations_function:
-		forall items found, found = find_obligations_function items
-		-> Forall P (use found) -> Forall P items.
-	Proof. intros ?[]; auto. Qed.
-
-End find_obligations.
-
-
-Module test__find_obligations.
-	Definition P n := n < 4 \/ n < 6.
-	Definition compute_partial: forall n, partial (P n).
-		refine (fun n => if (lt_dec n 4) then (Done _) else Undone); unfold P; lia.
-	Defined.
-
-	Definition items := [0; 1; 2; 4; 3; 2; 5].
-	Theorem items__find_obligations: Forall P items.
-	Proof.
-let pf := constr:(find_obligations_function P compute_partial items) in
-pose pf.
-
-
-let pf := eval compute in (find_obligations_function P compute_partial items) in
-idtac pf;
-pose (proj2_sig pf).
-let obligations := eval compute in (proj1_sig pf) in
-pose obligations;
-let H := eval compute in () in
-pose H.
-
-let i := fresh "obligations" in
-generalize .
-pose obligations.
-
-
-idtac.
-
-
-		find_obligations compute_partial items.
-apply s.
-let yo := eval compute in (proj1_sig s) in idtac.
-
-eval compute in (use s).
-apply o.
-apply Forall_fold_right; simpl; repeat split.
-
-
-simpl.
-
-End test__find_obligations.
-
-
-Ltac find_obligations compute_partial items :=
-	match goal with
-	| [ |- Forall ?P ?items] =>
-		let obligations := eval compute in (find_obligations_function P compute_partial items) in
-		pose obligations
-		(*; destruct obligations as [f o]*)
-		apply (use_find_obligations_function yo)
-		(*remember () as H;*)
-		(*destruct H as [? H]; apply H;*)
-		(*apply Forall_fold_right; simpl; repeat split*)
-		(*;
-		idtac;
-		apply Forall_fold_right; simpl; repeat split*)
-	(*Forall_forall*)
-	(*Forall_nth*)
-	(*Forall_lookup*)
-	(*Forall_lookup_total*)
-	end.
-
-
-
-Theorem append_single_cons {T: Type}: forall (t: T) l, t :: l = [t] ++ l.
-Proof. induction l; auto. Qed.
-
-Theorem valid_index_not_None {T} (l: list T) index:
-	index < (length l) -> (lookup index l) <> None.
-Proof.
-	intros ??%lookup_ge_None; lia.
-Qed.
-Theorem valid_index_Some {T} (l: list T) index:
-	index < (length l) -> exists t, (lookup index l) = Some t.
-Proof.
-	intros ?%(lookup_lt_is_Some_2 l index);
-	unfold is_Some in *; assumption.
-Qed.
-(*lookup_lt_Some*)
-Definition safe_lookup {T} index (l: list T):
-	index < (length l) -> {t | (lookup index l) = Some t}
-.
-	intros ?%valid_index_not_None;
-	destruct (lookup index l) eqn:Hlook; try contradiction;
-	rewrite <- Hlook; apply (exist _ t Hlook).
-Defined.
-
-
-Definition closer_to target: nat -> nat -> Prop :=
-	fun next cur => (target - next) < (target - cur).
-(*Hint Unfold closer_to: core.*)
-
-Theorem closer_to_well_founded target: well_founded (closer_to target).
-Proof.
-	apply (well_founded_lt_compat nat (fun a => target - a)); intros; assumption.
-Defined.
-
-Theorem closer_to_reverse: forall target cur next,
-	(target - next) < (target - cur) -> cur < next.
-Proof. lia. Qed.
-
-Theorem closer_to_bounded_reverse: forall target cur next,
-	cur < next -> cur < target -> (target - next) < (target - cur).
-Proof. lia. Qed.
-
-Definition closer_to_end {T} (arr: list T) := closer_to (length arr).
-
-Theorem closer_to_end_well_founded {T} (arr: list T): well_founded (closer_to_end arr).
-Proof. apply closer_to_well_founded. Qed.
+Require Import theorems.utils.
 
 Example test__vec_total_lookup: ([# 4; 2] !!! 0%fin) = 4.
 Proof. reflexivity. Qed.
-
-Theorem numeric_capped_incr_safe total begin cap index:
-	total = begin + cap
-	-> 0 < cap
-	-> index < begin
-	-> S index < total.
-Proof. lia. Qed.
-
-Theorem capped_incr_safe {T} (total begin cap: list T) index:
-	total = begin ++ cap
-	-> 0 < length cap
-	-> index < length begin
-	-> S index < length total.
-Proof.
-	intros Htotal Hcap Hindex;
-	assert (Hlen: length total = (length begin) + (length cap))
-		by solve [rewrite Htotal; apply app_length];
-	apply (numeric_capped_incr_safe Hlen Hcap Hindex).
-Qed.
-
-(*
-app_length: (l l': list A), length (l ++ l') = length l + length l'
-last_length: (l: list A) (a: A), length (l ++ [a]) = S (length l)
-*)
 
 Section Sized.
 	Variable size: nat.
@@ -241,7 +27,6 @@ Section Sized.
 		end
 	.
 
-	(*Definition label := option string.*)
 	Inductive Instruction :=
 		| InstExit
 		| InstMov (src: Operand) (dest: register)
@@ -334,12 +119,11 @@ Section Sized.
 	.*)
 
 	Theorem step_always_Within program cur next:
-		@step program cur next
-		-> Within program cur.
+		@step program cur next -> Within program cur.
 	Proof.
 		inversion 1;
 		match goal with
-		| [ H: _ !! counter _ = Some _ |- _ ] =>
+		| H: _ !! counter _ = Some _ |- _ =>
 			apply lookup_lt_Some in H; assumption
 		end.
 	Qed.
@@ -427,23 +211,28 @@ Section Sized.
 	Notation WellFormed program :=
 		(forall cur next, @step program cur next -> Within program next).
 
-	Definition partialOut (P: Prop) (x: partial P) :=
-		match x return (match x with | Proved _ => P | Uncertain => True end) with
-		| Proved pf => pf
-		| Uncertain => I
-		end
-	.
+	Definition check_instruction_well_formed index len_program: forall instr, partial (
+		forall program cur next,
+		(lookup index program) = Some instr
+		-> @step program cur next
+		-> cur.(counter) = index
+		-> len_program <= (length program)
+		-> Within program next
+	).
+		refine (fun instr =>
+			if (is_stopping instr) then found
+			else if (lt_dec (S index) len_program) then found else notfound
+			(*if (is_sequential instr)*)
+		);
+		intros ??? Hsome Hstep ??; subst;
+		try apply (stopping_stuck s Hsome) in Hstep;
+		destruct instr; inversion Hstep; try contradiction; simpl in *; subst; lia.
+	Defined.
 
-	Definition check_instruction_well_formed: forall instr index len_program,
-		{
-			forall program cur next,
-			(lookup program index) = Some instr
-			-> @step program cur next
-			-> cur.(counter) = index
-			-> len_program <= (length program)
-			-> Within program next
-		} + {}
-	.
+
+	Definition check_program_well_formed program :=
+		find_obligations (fun instr => ) (check_instruction_well_formed)
+		check_program_well_formed
 
 	Definition check_program_well_formed: list Instruction -> partial (WellFormed program).
 		refine (fun program =>
@@ -460,7 +249,7 @@ Section Sized.
 
 	Ltac program_well_formed :=
 		match goal with
-		| [ |- WellFormed ?program] => exact (partialOut (check_program_well_formed program))
+		| |- WellFormed ?program => exact (partialOut (check_program_well_formed program))
 		end.
 
 	Definition execute_program_unknown_termination
@@ -681,3 +470,4 @@ Inductive Result (T: Type) (E: Type): Type :=
 
 Arguments Ok {T} {E} _.
 Arguments Err {T} {E} _.
+
