theorems/utils.v
@@ -1,0 +1,233 @@
+Add LoadPath "/home/blaine/lab/cpdtlib" as Cpdt.
+Set Implicit Arguments. Set Asymmetric Patterns.
+Require Import List Cpdt.CpdtTactics.
+From stdpp Require Import base fin vector options.
+Import ListNotations.
+
+Ltac solve_crush := try solve [crush].
+Ltac solve_assumption := try solve [assumption].
+Ltac subst_injection H := injection H; intros; subst; clear H.
+
+Notation impossible := (False_rect _ _).
+Notation this item := (exist _ item _).
+Notation use item := (proj1_sig item).
+
+Section convert_subset.
+	Variable T: Type.
+	Variable P Q: T -> Prop.
+	Theorem convert_subset: {t | P t} -> (forall t: T, P t -> Q t) -> {t | Q t}.
+	Proof. intros []; eauto. Qed.
+End convert_subset.
+Arguments convert_subset {T} {P} {Q} _ _.
+
+Notation convert item := (convert_subset item _).
+
+Notation Yes := (left _ _).
+Notation No := (right _ _).
+Notation Reduce x := (if x then Yes else No).
+
+Theorem append_single_cons {T: Type}: forall (t: T) l, t :: l = [t] ++ l.
+Proof. induction l; auto. Qed.
+
+Theorem valid_index_not_None {T} (l: list T) index:
+	index < (length l) -> (lookup index l) <> None.
+Proof.
+	intros ??%lookup_ge_None; lia.
+Qed.
+Theorem valid_index_Some {T} (l: list T) index:
+	index < (length l) -> exists t, (lookup index l) = Some t.
+Proof.
+	intros ?%(lookup_lt_is_Some_2 l index);
+	unfold is_Some in *; assumption.
+Qed.
+(*lookup_lt_Some*)
+Definition safe_lookup {T} index (l: list T):
+	index < (length l) -> {t | (lookup index l) = Some t}
+.
+	intros ?%valid_index_not_None;
+	destruct (lookup index l) eqn:Hlook; try contradiction;
+	rewrite <- Hlook; apply (exist _ t Hlook).
+Defined.
+
+Theorem safe_lookup_In {T} index (l: list T) (H: index < length l):
+	In (use (safe_lookup l H)) l.
+Proof.
+	apply elem_of_list_In; destruct (safe_lookup l H); simpl;
+	apply elem_of_list_lookup; exists index; assumption.
+Qed.
+
+Theorem Forall_safe_lookup {T} (P: T -> Prop) l:
+	Forall P l <-> forall index (H: index < length l), P (use (safe_lookup l H)).
+Proof.
+	split.
+	-
+		intros; destruct (safe_lookup l _); simpl;
+		apply (Forall_lookup_1 P l index); assumption.
+	-
+		intros ?Hfunc; apply Forall_lookup; intros index item Hlookup;
+		specialize (lookup_lt_Some l index item Hlookup) as Hindex;
+		specialize (Hfunc index Hindex);
+		destruct (safe_lookup l _) as [item' Hitem'] in Hfunc; simpl in Hfunc;
+		rewrite Hlookup in Hitem'; subst_injection Hitem'; assumption.
+Qed.
+
+Definition closer_to target: nat -> nat -> Prop :=
+	fun next cur => (target - next) < (target - cur).
+(*Hint Unfold closer_to: core.*)
+
+Theorem closer_to_well_founded target: well_founded (closer_to target).
+Proof.
+	apply (well_founded_lt_compat nat (fun a => target - a)); intros; assumption.
+Defined.
+
+Theorem closer_to_reverse: forall target cur next,
+	(target - next) < (target - cur) -> cur < next.
+Proof. lia. Qed.
+
+Theorem closer_to_bounded_reverse: forall target cur next,
+	cur < next -> cur < target -> (target - next) < (target - cur).
+Proof. lia. Qed.
+
+Definition closer_to_end {T} (arr: list T) := closer_to (length arr).
+
+Theorem closer_to_end_well_founded {T} (arr: list T): well_founded (closer_to_end arr).
+Proof. apply closer_to_well_founded. Qed.
+
+Theorem numeric_capped_incr_safe total begin cap index:
+	total = begin + cap
+	-> 0 < cap
+	-> index < begin
+	-> S index < total.
+Proof. lia. Qed.
+
+Theorem capped_incr_safe {T} (total begin cap: list T) index:
+	total = begin ++ cap
+	-> 0 < length cap
+	-> index < length begin
+	-> S index < length total.
+Proof.
+	intros Htotal Hcap Hindex;
+	assert (Hlen: length total = (length begin) + (length cap))
+		by solve [rewrite Htotal; apply app_length];
+	apply (numeric_capped_incr_safe Hlen Hcap Hindex).
+Qed.
+
+
+Inductive partial (P: Prop): Type :=
+	| Found: P -> partial P
+	| NotFound: partial P
+.
+Notation found := (Found _).
+Notation notfound := (NotFound _).
+
+Section find_obligations.
+	Context {T: Type}.
+	Variable P: T -> Prop.
+
+	Theorem forall_done_undone items done undone:
+		Permutation items (done ++ undone)
+		-> Forall P done -> Forall P undone
+		-> Forall P items.
+	Proof.
+		intros Hpermutation??; assert (Happ: Forall P (done ++ undone))
+			by solve [apply Forall_app_2; assumption];
+		setoid_rewrite Hpermutation; assumption.
+	Qed.
+
+	Variable compute_partial: forall t: T, partial (P t).
+
+	Definition split_by_maybe: forall items: list T, {
+		pair | Permutation items (pair.1 ++ pair.2) /\ Forall P pair.1
+	}.
+		refine (fix split_by_maybe items :=
+			match items with
+			| [] => this ([], [])
+			| item :: items' =>
+				let (pair, H) := split_by_maybe items' in
+				match (compute_partial item) with
+				| Found _ => this ((item :: pair.1), pair.2)
+				| NotFound => this (pair.1, (item :: pair.2))
+				end
+			end
+		);
+		intros; split; simpl in *; try destruct H;
+		try solve [setoid_rewrite H; apply Permutation_middle]; auto.
+	Defined.
+
+	Definition find_obligations_function: forall items, {
+		obligations | Forall P obligations -> Forall P items
+	}.
+		refine (fun items =>
+			let (pair, H) := split_by_maybe items in
+			this pair.2
+		);
+		destruct H; apply (forall_done_undone H); assumption.
+	Defined.
+
+	Theorem verify__find_obligations_function:
+		forall items found, found = find_obligations_function items
+		-> Forall P (use found) -> Forall P items.
+	Proof. intros ?[]; auto. Qed.
+
+End find_obligations.
+
+Ltac find_obligations__helper P compute_partial items :=
+	let found := eval compute in (find_obligations_function P compute_partial items) in
+	let pf := eval compute in (proj2_sig found) in
+	apply pf; apply Forall_fold_right; simpl; repeat split
+.
+
+Ltac find_obligations P compute_partial items :=
+	match goal with
+	| |- Forall P items =>
+		find_obligations__helper P compute_partial items
+
+	| |- forall item, In item items -> P item =>
+		apply Coq.Lists.List.Forall_forall;
+		find_obligations__helper P compute_partial items
+
+	| |- forall item, elem_of item items -> P item =>
+		apply Forall_forall;
+		find_obligations__helper P compute_partial items
+
+	| |- forall index def, index < length items -> P (nth index items def) =>
+		apply Coq.Lists.List.Forall_nth;
+		find_obligations__helper P compute_partial items
+
+	| |- forall index item, (lookup index items) = Some item -> P item =>
+		apply Forall_lookup;
+		find_obligations__helper P compute_partial items
+
+	| |- forall index, index < length items -> P (items !!! index) =>
+		apply Forall_lookup_total;
+		find_obligations__helper P compute_partial items
+
+	| |- forall index (H: index < length items), P (use (safe_lookup items H)) =>
+		apply Forall_safe_lookup;
+		find_obligations__helper P compute_partial items
+	end
+.
+
+Module test__find_obligations.
+	Definition P n := (n < 4 \/ n < 6).
+	Definition compute_partial: forall n, partial (P n).
+		refine (fun n => if (lt_dec n 4) then found else notfound); unfold P; lia.
+	Defined.
+
+	Definition items := [0; 1; 2; 4; 3; 2; 5].
+	Theorem find_obligations__Forall: Forall P items.
+	Proof. find_obligations P compute_partial items; lia. Qed.
+	Theorem find_obligations__forall_In: forall item, In item items -> P item.
+	Proof. find_obligations P compute_partial items; lia. Qed.
+	Theorem find_obligations__forall_elem_of: forall item, elem_of item items -> P item.
+	Proof. find_obligations P compute_partial items; lia. Qed.
+	Theorem find_obligations__forall_nth: forall index def, index < length items -> P (nth index items def).
+	Proof. find_obligations P compute_partial items; lia. Qed.
+	Theorem find_obligations__forall_lookup: forall index item, (lookup index items) = Some item -> P item.
+	Proof. find_obligations P compute_partial items; lia. Qed.
+	Theorem find_obligations__forall_lookup_total: forall index, index < length items -> P (items !!! index).
+	Proof. find_obligations P compute_partial items; lia. Qed.
+	Theorem find_obligations__forall_safe_lookup:
+		forall index (H: index < length items), P (use (safe_lookup items H)).
+	Proof. find_obligations P compute_partial items; lia. Qed.
+End test__find_obligations.
